CheriDecExec.v
@@ -1,0 +1,60 @@
+Require Import Kami.AllNotations ProcKami.CheriTypes ProcKami.Lib.
+
+Section DecExec.
+  Context `{procParams: ProcParams}.
+  Variable ty: Kind -> Type.
+  Local Open Scope kami_expr.
+
+  Variable pc: FullCap @# ty.
+  Variable inst: Inst @# ty.
+  Variable cs1: FullCapWithTag @# ty.
+  Variable cs2: FullCapWithTag @# ty.
+  Variable scr: FullCapWithTag @# ty.
+  Variable csr: Data @# ty.
+  Variable ie: Bool @# ty.
+
+  Definition matchField (f: FieldRange) :=
+    let '(existT (start, size) field) := f in
+    UniBit (TruncMsb start size) (ZeroExtendTruncLsb (start + size) inst) ==
+      Const ty field.
+
+  Definition matchUniqId (uid: UniqId) :=
+    CABool And (map matchField uid).
+
+  Section Decode.
+    Variable decOutput: Kind.
+    Local Fixpoint decodeHelp (ls: list (InstEntry decOutput)) (exprs: list (decOutput @# ty)) : decOutput ## ty :=
+      match ls with
+      | nil => RetE (Kor exprs)
+      | i :: rest => ( LETE decI <- inputXform i pc inst cs1 cs2 scr csr ie;
+                       LETC matchI <- matchUniqId (uniqId i);
+                       decodeHelp rest (ITE #matchI #decI (Const ty Default) :: exprs) )
+      end.
+
+    Definition decode (ls: list (InstEntry decOutput)) := decodeHelp ls [].
+    
+    Definition decodeMatch (ls: list (InstEntry decOutput)) :=
+      Kor (map (fun i => matchUniqId (uniqId i)) ls).
+  End Decode.
+
+  Definition funcEntryExec (funcEntry: FuncEntry) (decOut: localFuncInput funcEntry ## ty) : FuncOutput ## ty :=
+    ( LETE decOutput <- decOut;
+      LETC decMatch <- decodeMatch (insts funcEntry);
+      LETE fuOut <- localFunc funcEntry #decOutput;
+      LETE execOut <- outputXform funcEntry #fuOut;
+      RetE (ITE #decMatch #execOut (Const ty Default)) ).
+
+  Definition fullDec (ls: list FuncEntry) := map (fun f => existT _ f (decode (insts f))) ls.
+
+  Local Fixpoint fullExecHelp (ls: list {f: FuncEntry & localFuncInput f ## ty } )
+    (exprs: list (FuncOutput @# ty)) : FuncOutput ## ty :=
+    match ls with
+    | nil => RetE (Kor exprs)
+    | existT f decOut :: rest => ( LETE execOut <- funcEntryExec f decOut;
+                                   fullExecHelp rest (#execOut :: exprs) )
+    end.
+
+  Definition fullExec (ls: list {f: FuncEntry & localFuncInput f ## ty }) := fullExecHelp ls [].
+
+  Definition fullDecExec (ls: list FuncEntry) := fullExec (fullDec ls).
+End DecExec.
